{
 "cells": [
  {
   "cell_type": "markdown",
   "id": "12df79c4",
   "metadata": {},
   "source": [
    "# <center>Math 589 Homework2 Solution<center>\n",
    "<center>Yuan Yin A20447290</center>"
   ]
  },
  {
   "cell_type": "markdown",
   "id": "1c1ea6f2",
   "metadata": {},
   "source": [
    "## Question 1\n",
    "Find the local trunction error of the difference equation\n",
    "\\begin{equation}\\label{FTBS.numsol}\n",
    "    U_j^{n+1}=U_j^n-R(U_j^n-U_{j-1}^n)\n",
    "\\end{equation}\n",
    "for the PDE\n",
    "\\begin{equation}\\label{PDE.anasol}\n",
    "    u_t+au_x=0,\\quad 0\\le x\\le 1,t>0,\n",
    "\\end{equation}\n",
    "where $R=a\\Delta t/\\Delta x$ and $a>0$ is a constant.\n",
    "\n",
    "**proof:**\n",
    "By the definition of truncation error at grid point $(x_j,t_n)$, denoted as $T_j^n$:\n",
    "\\begin{equation}\\label{trun.error}\n",
    "    T_j^n:=u(x_j,t_{n+1})-u(x_j,t_n)+R(u(x_j,t_n)-u(x_{j-1},t_n)).\n",
    "\\end{equation}\n",
    "\n",
    "Then using Taylor expansion, we have the following two equations:\n",
    "\\begin{align*}\n",
    "    u(x_j,t_{n+1})&=u(x_j,t_n+\\Delta t)=u(x_j,t_n)+ u_t(x_j,t_n)\\Delta t+\\frac{1}{2}u_{tt}(x_j,\\eta)(\\Delta t)^2,\\quad \\eta\\in(t_n,t_{n+1}).\\\\\n",
    "    u(x_{j-1},t_n)&=u(x_j-\\Delta x,t_n)=u(x_j,t_n)-u_x(x_j,t_n)\\Delta x+\\frac{1}{2}u_{xx}(\\xi,t_n)(\\Delta x)^2,\\quad\\xi\\in(x_{j-1},x_j).\\\\\n",
    "\\end{align*}\n",
    "\n",
    "Plug the two equations above into truncation error equation \\eqref{trun.error}, we get\n",
    "\\begin{align*}\n",
    "    T_j^n&=u_t(x_j,t_n)\\Delta t+\\frac{1}{2}u_{tt}(x_j,\\eta)(\\Delta t)^2+R\\left(u_x(x_j,t_n)\\Delta x-\\frac{1}{2}u_{xx}(\\xi,t_n)(\\Delta x)^2\\right)\\\\\n",
    "    &=\\Delta t\\left(u_t(x_j,t_n)+au_x(x_j,t_n)\\right)+\\frac{1}{2}u_{tt}(x_j,\\eta)(\\Delta t)^2-\\frac{a\\Delta t\\Delta x}{2}u_{xx}(\\xi,t_n),\\quad\\text{since $R=a\\Delta t/\\Delta x$}\\\\\n",
    "    &=\\frac{1}{2}u_{tt}(x_j,\\eta)(\\Delta t)^2-\\frac{a\\Delta t\\Delta x}{2}u_{xx}(\\xi,t_n),\\quad\\text{since \\eqref{PDE.anasol}}\n",
    "\\end{align*}\n",
    "\n",
    "## Question 2\n",
    "**proof:**\n",
    "Suppose:\n",
    "\\begin{equation*}\n",
    "U_j^n=u(x_j,t_n)+e_j^n.\n",
    "\\end{equation*}\n",
    "By definition, FTBS scheme converges if $e_j^n\\to 0$ as $(\\Delta x,\\Delta t)\\to 0$.\n",
    "\n",
    "Plug the equation above into equation \\eqref{FTBS.numsol}, we get\n",
    "\\begin{align*}\n",
    "&u(x_j,t_n)+e_j^n=u(x_j,t_{n+1})+e_j^{n+1}+R\\left(u(x_j,t_n)+e_j^n-u(x_{j-1},t_n)-e_{j-1}^n\\right)\\\\\n",
    "&\\Rightarrow e_j^{n+1}=(1-R)e_j^n+Re_{j-1}^n-\\left(u(x_j,t_{n+1})-u(x_j,t_n)+R\\left(u(x_j,t_n)-u(x_{j-1},t_n)\\right)\\right)\\\\\n",
    "&\\Rightarrow e_j^{n+1}=(1-R)e_j^n+Re_{j-1}^n-T_j^n.\n",
    "\\end{align*}\n",
    "\n",
    "From the results of question 1, we know that\n",
    "\\begin{align*}\n",
    "    |T_j^n|&=\\left|\\frac{1}{2}M_{tt}(\\Delta t)^2-\\frac{a\\Delta t\\Delta x}{2}M_{xx}=\\left(\\frac{1}{2}M_{tt}(\\frac{\\Delta t}{\\Delta x})^2-\\frac{a\\Delta t}{2\\Delta x}M_{xx}\\right)(\\Delta x)^2\\right|\\\\\n",
    "    &=\\left|\\left(\\frac{1}{2}M_{tt}(\\frac{\\Delta t}{\\Delta x})^2-\\frac{a\\Delta t}{2\\Delta x}M_{xx}\\right)(\\Delta x)^2\\right|\\\\\n",
    "    &=\\left|\\left(\\frac{1}{2}M_{tt}R^2-\\frac{a}{2}M_{xx}R\\right)(\\Delta x)^2\\right|\\\\\n",
    "    &\\le M(\\Delta x)^2\n",
    "\\end{align*}\n",
    "where $M>0$ is a constant.\n",
    "\n",
    "Additionally, suppose $E^n:=\\max_j{|e_j^n|}$ and knowing that $R\\in(0,1],1-R\\in[0,1)$. Then\n",
    "\\begin{align*}\n",
    "    |e_j^n|&\\le E^{n+1}\\le (1-R)E^n+RE^n+M(\\Delta x)^2\\\\\n",
    "    &\\le E^{n-1}+2M(\\Delta x)^2\\le\\dots\\le E^0+(n+1)M(\\Delta x)^2\\to 0 \\quad\\text{as $(\\Delta x,\\Delta t)\\to 0$}.\n",
    "\\end{align*}\n",
    "Convergence proved.\n",
    "\n",
    "## Question 3\n",
    "**proof:**\n",
    "Assume the solution has the form $U_j^n=\\lambda^ne^{ik(j\\Delta x)}$.\n",
    "\n",
    "Plug the solution above into FTBS scheme in equation \\eqref{FTBS.numsol}:\n",
    "\\begin{align*}\n",
    "    &\\lambda^{n+1}e^{ik(j\\Delta x)}=\\lambda^ne^{ik(j\\Delta x)}-R(\\lambda^ne^{ik(j\\Delta x)}-\\lambda^ne^{ik(j-1)\\Delta x})\\\\\n",
    "    &\\Rightarrow\\lambda=1-R+R\\cos(k\\Delta x)-iR\\sin(k\\Delta x)\\\\\n",
    "    &\\Rightarrow|\\lambda|=(1-R+R\\cos(k\\Delta x))^2+R\\sin^2(k\\Delta x)\\\\\n",
    "    &\\Rightarrow|\\lambda|=(2R^2-2R)(1-\\cos(k\\Delta x))+1.\n",
    "\\end{align*}\n",
    "\n",
    "To satisfy the stability condition, we have\n",
    "\\begin{align*}\n",
    "    &|\\lambda|\\le 1\\\\\n",
    "    &\\Rightarrow(2R^2-2R)(1-\\cos(k\\Delta x))\\le 0\\\\\n",
    "    &\\Rightarrow 0\\le R\\le 1\\\\\n",
    "\\end{align*}\n",
    "\n",
    "Since by definition, $R:=a\\Delta t/\\Delta x>0$, the necessary stability condition of the FTBS scheme \\eqref{FTBS.numsol} is $R\\in(0,1]$."
   ]
  }
 ],
 "metadata": {
  "kernelspec": {
   "display_name": "Python 3",
   "language": "python",
   "name": "python3"
  },
  "language_info": {
   "codemirror_mode": {
    "name": "ipython",
    "version": 3
   },
   "file_extension": ".py",
   "mimetype": "text/x-python",
   "name": "python",
   "nbconvert_exporter": "python",
   "pygments_lexer": "ipython3",
   "version": "3.8.8"
  }
 },
 "nbformat": 4,
 "nbformat_minor": 5
}
